first lemma proof

coq/TM.v
@@ -77,11 +77,77 @@ Fixpoint is_access {S} (cfgs : @tm_configuration S) (ast : @states S) :=
   | _, _ => False
   end.
 
+Definition command_right_form {S} (A : Type) (cmd : @command S) := 
+  match cmd with
+  | (l1, s1, r1) -> (l2, s2, r2) =>
+      r1 <> LeftBounding /\ r2 <> LeftBounding /\ l1 <> RightBounding /\ l2 <> RightBounding /\
+      (r1 = r2 /\ (l1 = l2 \/ r1 = RightBounding /\ l1 <> LeftBounding /\ l2 <> LeftBounding) \/
+      (exists (a1 a2 a3 a4 : A), l1 = L/a1 /\ l2 = L/a2 /\ r1 = L/a3 /\ r2 = L/a4))
+  end.
+
+Definition command_applicable {S} (A : Type) (cmd : @command S) (cfg : @config S) :=
+  match cmd, cfg with
+  | (l1, s1, r1) -> (l2, s2, r2), Config l s r => 
+      s1 = s /\ 
+      (l1 = Empty /\ r1 = RightBounding /\ r = [r1] \/
+      r1 = RightBounding /\ r = [r1] /\ l2 = Empty /\ l1 = (last l LeftBounding) \/
+      (exists (a1 a2 : A), l1 = L/a1 /\ r1 = L/a2 /\ (last l LeftBounding) = l1 /\ (hd RightBounding r) = r1))
+  end.
+
+Compute last [] 5.
+Compute hd 3 [].
+
+Definition apply_command {S} (cmd : @command S) (cfg : @config S) :=
+  match cmd, cfg with
+  | (l1, s1, r1) -> (l2, s2, r2), Config l s r => 
+    match l1, l2 with
+    | Empty, Empty => Config l s2 r
+    | Empty, _ => Config (l ++ [l2]) s2 r
+    | _, Empty => Config (removelast l) s2 r
+    | _, _ => Config ((removelast l) ++ [l2]) s2 (r2 :: (tl r))
+    end
+  end.
+
+Lemma next_cfg_exists : forall (A S : Type) (cmd : @command S) (cfg : @config S),
+  command_right_form A cmd /\ command_applicable A cmd cfg ->
+  (exists new_cfg, apply_command cmd cfg = new_cfg).
+Proof.
+  intros A S cmd cfg [H1 H2].
+  destruct cmd. destruct t1. destruct t2. destruct cfg.
+  unfold command_right_form in H1.
+  unfold command_applicable in H2.
+  unfold apply_command.
+  destruct H1 as [H0 [H1 [H3 [H4 [[H5 [H6|H6]]|H5]]]]].
+  - destruct H2 as [H2 [[H7 [H8 H9]]|[[H7 [H8 [H9 H10]]]|[a1 [a2 [H7 [H8 [H9 H10]]]]]]]].
+    + subst. exists (Config l1 s0 [RightBounding]). reflexivity.
+    + subst. exists (Config l1 s0 [RightBounding]). reflexivity.
+    + subst. exists (Config (removelast l1 ++ [Letter a1]) s0 (Letter a2 :: tl r1)). reflexivity.
+  - destruct H2 as [H2 [[H7 [H8 H9]]|[[H7 [H8 [H9 H10]]]|[a1 [a2 [H7 [H8 [H9 H10]]]]]]]].
+    + subst. destruct l0.
+      * destruct H4. reflexivity.
+      * destruct H6 as [_ [_ []]]. reflexivity.
+      * exists (Config l1 s0 [RightBounding]). reflexivity.
+      * exists (Config (l1 ++ [Letter a]) s0 [RightBounding]). reflexivity.
+    + subst. destruct (last l1 LeftBounding).
+      * simpl. destruct H3. reflexivity.
+      * destruct H6 as [_ [H6]]. destruct H6. reflexivity.
+      * exists (Config l1 s0 [RightBounding]). reflexivity.
+      * exists (Config (removelast l1) s0 [RightBounding]). reflexivity.
+    + subst. destruct l0.
+      * destruct H4. reflexivity.
+      * destruct H6 as [_ [_ []]]. reflexivity.
+      * exists (Config (removelast l1) s0 r1). reflexivity.
+      * destruct H6 as [H6 _]. discriminate H6.
+  - destruct H2 as [H2 [[H7 [H8 H9]]|[[H7 [H8 [H9 H10]]]|[a5 [a6 [H7 [H8 [H9 H10]]]]]]]]; 
+    destruct H5 as [a1 [a2 [a3 [a4 [H5 [H11 [H12 H13]]]]]]]; subst; try discriminate.
+    + exists (Config (removelast l1 ++ [Letter a2]) s0 (Letter a4 :: tl r1)). reflexivity.
+  Qed.
+
 (*
-s1 == s && 
-(r1 == emptySymbol && l1 == rightBoundingLetter && l2 == l1 && l == [] ||
-r1 == (last r emptySymbol) && l1 == rightBoundingLetter && r2 == emptySymbol && l2 == l1 && l == [] ||
-(last r) == r1 && (hd emptySymbol l) == l1 && r2 <> leftBoundingLetter && l2 <> rightBoundingLetter) -> checkCommandTapeToTape t2 t1
+((l1, s1, r1) -> (l2, s2, r2)) : t1, (l, s, r) : t2) => s1 = s /\ 
+  (l1 = Empty /\ r1 = RightBounding /\ r = [r1] \/
+  l <> [LeftBounding] /\ l1 = (last l) /\ r1 = RightBounding /\ l2 = Empty /\ r2 = r1 /\ r = [r1] \/
+  (last l) = l1 /\ (head r) = r1) /\ checkCommandTapeToTape t2 t1
 *)
 
 Fixpoint get_applicable_cmds {A S} (cfgs : @tm_configuration A S) (cmds : list (list (@command A S))) 
